json/Theorems/Utf8.v
@@ -9,6 +9,54 @@ Require Import Json.Utf8.
 
 Open Scope string_scope.
 
+Ltac destruct_parse_continuation :=
+  match goal with
+    | [G: context[parse_continuation (?a::?b) = Ok (?resp, ?suffix)] |- _] => idtac
+    | [H: context[parse_continuation ?text = Ok (?resp, ?suffix)] |- _] => destruct text; [ discriminate H | ]
+  end;
+  match goal with
+    | [H: context[parse_continuation (?b::?rest) = Ok (?resp, ?suffix)] |- _] =>
+        unfold parse_continuation in H;
+        rewrite parser_map_correct in H;
+        simpl in H;
+        let B1 := fresh "b" in
+        let B2 := fresh "b" in
+        let B3 := fresh "b" in
+        let B4 := fresh "b" in
+        let B5 := fresh "b" in
+        let B6 := fresh "b" in
+        let B7 := fresh "b" in
+        let B8 := fresh "b" in
+        let eqn_name := fresh "byte_bits" in
+        destruct (Byte.to_bits b) as [B1 [B2 [B3 [B4 [B5 [B6 [B7 B8]]]]]]] eqn:eqn_name;
+        match goal with
+        | [G: context[if (?a && negb ?b) then _ else _] |- _ ] =>
+            destruct a; destruct b; try discriminate G; simpl in H; rewrite eqn_name in H;
+            apply (f_equal Byte.of_bits) in eqn_name;
+            rewrite Byte.of_bits_to_bits in eqn_name
+        end
+    end.
+
+Ltac to_bits byte :=
+  let rec break_bit bits :=
+    match type of bits with
+    | (bool * bool)%type => let b1 := fresh "b" in let b2 := fresh "b" in destruct bits as [b1 b2]
+    | (bool * ?rest)%type => let b := fresh "b" in destruct bits as [b _bits]; break_bit _bits
+    | (?rest * bool)%type => let b := fresh "b" in destruct bits as [_bits b]; break_bit _bits
+    | ?other => idtac other
+    end
+  in 
+  match type of byte with
+  | Utf8.b6 =>
+      unfold Utf8.b6 in byte; break_bit byte
+  | Byte.byte =>
+      let B := fresh "B" in
+      let eqn_name := fresh "byte_bits" in
+      remember (Byte.to_bits byte) as B eqn:eqn_name;
+      break_bit B;
+      symmetry in eqn_name
+  end.
+
 Lemma utf8_encode_correct : forall (c: codepoint) l,
     l = utf8_encode_codepoint c  ->
     (exists b1 b2 b3 b4 b5 b6 b7,
@@ -60,50 +108,88 @@ Ltac for_all_valid_utf8_encodings c :=
   in f encodings.
 
 Theorem encoding_size_correct :
-  (forall b1 b2 b3 b4 b5 b6 b7,
-      encoding_size_from_header
-        (Byte.of_bits (b1, (b2, (b3, (b4, (b5, (b6, (b7, false)))))))) = Some (OneByte (b7, b6, b5, b4, b3, b2, b1)))
-  /\ (forall b1 b2 b3 b4 b5,
-         encoding_size_from_header
-           (Byte.of_bits (b1, (b2, (b3, (b4, (b5, (false, (true, true)))))))) = Some (TwoBytes (b5, b4, b3, b2, b1)))
-  /\ (forall b1 b2 b3 b4,
-         encoding_size_from_header
-           (Byte.of_bits (b1, (b2, (b3, (b4, (false, (true, (true, true)))))))) = Some (ThreeBytes (b4, b3, b2, b1)))
-  /\ (forall b1 b2 b3,
-         encoding_size_from_header
-        (Byte.of_bits (b1, (b2, (b3, (false, (true, (true, (true, true)))))))) = Some (FourBytes (b3, b2, b1))).
+  (forall byte b1 b2 b3 b4 b5 b6 b7, byte = (Byte.of_bits (b1, (b2, (b3, (b4, (b5, (b6, (b7, false)))))))) <->
+      encoding_size_from_header byte = Some (OneByte (b7, b6, b5, b4, b3, b2, b1)))
+  /\ (forall byte b1 b2 b3 b4 b5, byte = (Byte.of_bits (b1, (b2, (b3, (b4, (b5, (false, (true, true)))))))) <->
+         encoding_size_from_header byte = Some (TwoBytes (b5, b4, b3, b2, b1)))
+  /\ (forall byte b1 b2 b3 b4, byte = (Byte.of_bits (b1, (b2, (b3, (b4, (false, (true, (true, true)))))))) <->
+         encoding_size_from_header byte = Some (ThreeBytes (b4, b3, b2, b1)))
+  /\ (forall byte b1 b2 b3, byte = (Byte.of_bits (b1, (b2, (b3, (false, (true, (true, (true, true)))))))) <->
+         encoding_size_from_header byte = Some (FourBytes (b3, b2, b1))).
 Proof.
-  unfold encoding_size_from_header.
-  repeat split; intros; rewrite Byte.to_bits_of_bits;
+  repeat (split; intros; subst);
+    try (unfold encoding_size_from_header; repeat rewrite Byte.to_bits_of_bits;
+         repeat match goal with
+           | [ |- (if ?bit then _ else _) = _ ] => destruct bit
+           | [ |- (_ = _)] => reflexivity
+           end);
+    unfold encoding_size_from_header in H;
+    to_bits byte;
+    apply (f_equal Byte.of_bits) in byte_bits;
+    rewrite Byte.of_bits_to_bits in byte_bits;
+    rewrite byte_bits;
     repeat match goal with
-      | [ |- (if ?bit then _ else _) = _ ] => destruct bit
-      | [ |- (_ = _)] => reflexivity
-    end.
+      | [ H: (if ?bit then _ else _) = _ |- _ ] => destruct bit
+      | [ |- (_ = _)] => try discriminate; inversion H; reflexivity
+      end.
 Defined.
 
-Theorem parse_continuation_correct: forall rest b1 b2 b3 b4 b5 b6,
-    parse_continuation (Byte.of_bits (b1, (b2, (b3, (b4, (b5, (b6, (false, true))))))) :: rest) = Ok ((b6, b5, b4, b3, b2, b1), rest).
+Lemma enc_one_spec: forall b1 b2 b3 b4 b5 b6 b7, encoding_size_from_header (Byte.of_bits (b1, (b2, (b3, (b4, (b5, (b6, (b7, false)))))))) = Some (OneByte (b7, b6, b5, b4, b3, b2, b1)).
 Proof.
   intros.
-  unfold parse_continuation.
-  rewrite parser_map_correct.
-  unfold predicate. rewrite Byte.to_bits_of_bits.
-  unfold fmap.
-  unfold bind.
-  assert ((if true && negb false
-     then Ok (Byte.of_bits (b1, (b2, (b3, (b4, (b5, (b6, (false, true))))))), rest)
-     else
-      Err
-        (Error
-           (InvalidContinuationHeader
-              (Some
-                 (Byte.of_bits
-                    (b1, (b2, (b3, (b4, (b5, (b6, (false, true)))))))))))) = Ok (Byte.of_bits (b1, (b2, (b3, (b4, (b5, (b6, (false, true))))))), rest)) as G; try reflexivity.
-  rewrite G.
-  rewrite Byte.to_bits_of_bits.
+  destruct encoding_size_correct as [e1 [e2 [e3 e4]]].
+  eapply e1. reflexivity.
+Defined.
+
+Lemma enc_two_spec: forall b1 b2 b3 b4 b5, encoding_size_from_header (Byte.of_bits (b1, (b2, (b3, (b4, (b5, (false, (true, true)))))))) = Some (TwoBytes (b5, b4, b3, b2, b1)).
+Proof.
+  intros.
+  destruct encoding_size_correct as [e1 [e2 [e3 e4]]].
+  eapply e2. reflexivity.
+Defined.
+
+Lemma enc_three_spec: forall b1 b2 b3 b4, encoding_size_from_header (Byte.of_bits (b1, (b2, (b3, (b4, (false, (true, (true, true)))))))) = Some (ThreeBytes (b4, b3, b2, b1)).
+Proof.
+  intros.
+  destruct encoding_size_correct as [e1 [e2 [e3 e4]]].
+  eapply e3. reflexivity.
+Defined.
+
+Lemma enc_four_spec: forall b1 b2 b3, encoding_size_from_header (Byte.of_bits (b1, (b2, (b3, (false, (true, (true, (true, true)))))))) = Some (FourBytes (b3, b2, b1)).
+Proof.
+  intros.
+  destruct encoding_size_correct as [e1 [e2 [e3 e4]]].
+  eapply e4. reflexivity.
+Defined.
+
+Theorem parse_continuation_correct: forall byte rest b1 b2 b3 b4 b5 b6,
+    parse_continuation (byte :: rest) = Ok ((b6, b5, b4, b3, b2, b1), rest) <-> byte = Byte.of_bits (b1, (b2, (b3, (b4, (b5, (b6, (false, true))))))).
+Proof.
+  intros. split; intros.
+  - destruct_parse_continuation. inversion H; subst. reflexivity.
+  - subst. unfold parse_continuation. rewrite parser_map_correct. unfold predicate. rewrite Byte.to_bits_of_bits. unfold fmap, bind. assert (true && negb false = true). reflexivity. rewrite H. rewrite Byte.to_bits_of_bits. reflexivity.
+Defined.
+
+Theorem parse_continuation_strong_progress: forall suffix response text,
+    (parse_continuation text = Ok (response, suffix)) ->
+    length suffix < length text.
+Proof.
+  intros.
+  generalize dependent response.
+  generalize dependent suffix.
+  induction text as [| byte1 text_rest]; intros.
+  - inversion H.
+  - destruct_parse_continuation. inversion H. subst.
+    simpl. lia.
+Defined.
+
+Lemma parse_continuation_spec: forall rest b1 b2 b3 b4 b5 b6, parse_continuation ((Byte.of_bits (b1, (b2, (b3, (b4, (b5, (b6, (false, true)))))))) :: rest) = Ok ((b6, b5, b4, b3, b2, b1), rest).
+Proof.
+  intros.
+  eapply parse_continuation_correct.
   reflexivity.
 Defined.
-  
+
 Theorem parse_codepoint_encode_correct : forall c rest, parse_codepoint ((utf8_encode_codepoint c) ++ rest)%list = Ok (c, rest).
 Proof.
 
@@ -115,14 +201,13 @@ Proof.
     end.
   
   intros.
-  destruct encoding_size_correct as [enc_one [enc_two [enc_three enc_four]]].
   for_all_valid_utf8_encodings c;
     auto;
     rewrite eq;
     unfold parse_codepoint, parse_header, bind, app;
-    [ rewrite enc_one | rewrite enc_two | rewrite enc_three | rewrite enc_four];
+    [ rewrite enc_one_spec | rewrite enc_two_spec | rewrite enc_three_spec | rewrite enc_four_spec];
     rewrite c_eq;
-    repeat rewrite parse_continuation_correct;
+    repeat rewrite parse_continuation_spec;
     try reflexivity;
     unfold codepoint_range_to_codepoint, bind;
     no_overlongs.
@@ -135,8 +220,14 @@ Proof.
   apply (parse_codepoint_encode_correct c []).
 Defined.
 
+Ltac no_overlong_encoding Hyp :=
+  repeat match type of Hyp with
+    | context[if ?bit then _ else _] => destruct bit
+    | Err _ = Ok _ => discriminate Hyp
+    end.
+
 Lemma parse_codepoint_strong_progress: forall suffix response text,
-    (Ok (response, suffix) = parse_codepoint text) ->
+    (parse_codepoint text = Ok (response, suffix)) ->
     length suffix < length text.
 Proof.
   intros.
@@ -144,10 +235,10 @@ Proof.
   generalize dependent suffix.
   induction text as [| byte1 text_rest1]; intros.
   - inversion H.
-  - simpl. (* apply Nat.lt_lt_succ_r. *)
-    destruct (Byte.to_bits byte1) as [b1 [b2 [b3 [b4 [b5 [b6 [b7 b8]]]]]]] eqn:byte1_bits.
+  - simpl. 
+    to_bits byte1.
     unfold parse_codepoint, parse_header, encoding_size_from_header in H.
-    rewrite byte1_bits in H.
+    rewrite byte_bits in H.
     repeat match goal with
            | [ H: context[if ?bit then _ else _] |- _ ] => destruct bit
            | [ H: (_ = _) |- _ ] => simpl in H; discriminate H
@@ -155,31 +246,17 @@ Proof.
       (* encoding size = 1 *)
       try (inversion H; lia);
       (* encoding size = 2 *)
-      unfold parse_continuation, predicate in H;
-      destruct text_rest1 as [| byte2 text_rest2] eqn:E_text_rest1; try (simpl in H; discriminate H);
-      rewrite parser_map_correct in H;
-      destruct (Byte.to_bits byte2) as [B1 [B2 [B3 [B4 [B5 [B6 [B7 B8]]]]]]] eqn:byte2_bits;
-      destruct B8; destruct B7; try discriminate H; simpl in H; rewrite byte2_bits in H;
-      try (simpl; inversion H; subst; lia);
+      destruct (parse_continuation text_rest1) as [[val1 text_rest2] | err] eqn:P_cont_text_rest1; try discriminate H;
+      destruct_parse_continuation; to_bits val1; inversion H; subst; inversion P_cont_text_rest1; subst; clear H; simpl; try lia;
+      no_overlong_encoding H1; inversion H1; try lia;
       (* encoding size = 3 *)
-      try (destruct text_rest2 as [| byte3 text_rest3] eqn:E_text_rest2; [
-            simpl in H; discriminate H |
-            rewrite parser_map_correct in H;
-            destruct (Byte.to_bits byte3) as [C1 [C2 [C3 [C4 [C5 [C6 [C7 C8]]]]]]] eqn:byte3_bits;
-            destruct C8; destruct C7; try discriminate H; simpl in H; rewrite byte3_bits in H
-        ]);
+      destruct (parse_continuation text_rest2) as [[val2 text_rest3] | err] eqn:P_cont_text_rest2; try discriminate H1;
+      destruct_parse_continuation; to_bits val2; inversion P_cont_text_rest2; inversion H1; subst; simpl; try lia;
+      no_overlong_encoding H9; inversion H9; try lia;
       (* encoding size = 4 *)
-      try (simpl; inversion H; subst; lia);
-      try (destruct text_rest3 as [| byte4 text_rest4] eqn:E_text_rest3; [
-        simpl in H; discriminate H |
-        rewrite parser_map_correct in H;
-        destruct (Byte.to_bits byte4) as [D1 [D2 [D3 [D4 [D5 [D6 [D7 D8]]]]]]] eqn:byte4_bits;
-        destruct D8; destruct D7; try discriminate H; simpl in H; rewrite byte4_bits in H
-      ]);
-      repeat match goal with
-        | [ H: context[if ?bit then _ else _] |- _ ] => destruct bit
-        | [ H: (_ = _) |- _ ] => simpl in H; try discriminate H; inversion H; simpl; lia
-        end.
+      destruct (parse_continuation text_rest3) as [[val3 text_rest4] | err] eqn:P_cont_text_rest3; try discriminate H9;
+      destruct_parse_continuation; to_bits val3; inversion P_cont_text_rest3; inversion H9; subst; simpl; try lia;
+      no_overlong_encoding H11; inversion H11; lia.
 Defined.
     
 Lemma many_codepoint_distributes : forall (c: codepoint) (cs: list codepoint),
@@ -210,48 +287,74 @@ Proof.
   reflexivity.
 Defined.
 
+Theorem decode_encode_correct_strong: forall (unicode: unicode_str) (bytes rest: list Byte.byte),
+    forall lesser, ((length lesser) <= (length bytes)) ->
+            (utf8_decode lesser = Ok (unicode, rest)) ->
+            lesser = List.app (utf8_encode unicode) rest.
+Proof.
+  intros unicode bytes.
+  generalize dependent unicode.
+  destruct encoding_size_correct as [e1 [e2 [e3 e4]]].
+  induction bytes; intros unicode rest lesser enough_fuel IH_bytes.
+  - inversion enough_fuel. Search (List.length). rewrite length_zero_iff_nil in H0. subst. inversion IH_bytes. reflexivity.
+  - unfold utf8_decode, many in IH_bytes. simpl in IH_bytes.
+    destruct (parse_codepoint lesser) as [[val rest1] | err] eqn:Parse_lesser; [| inversion IH_bytes; reflexivity].
+    destruct lesser as [| byte1 bytes_rest1].
+    + inversion Parse_lesser; reflexivity.
+    + unfold parse_codepoint, parse_header in Parse_lesser.
+      destruct (encoding_size_from_header byte1) as [enc_size| ] eqn:Enc_byte1; simpl in Parse_lesser; [| inversion Parse_lesser; reflexivity].
+      destruct enc_size as [ [[[[[[b7 b6] b5] b4]b3] b2] b1]| [[[[b11 b10] b9] b8] b7] | [[[b16 b15] b14] b13] | [[b21 b20] b19] ] eqn:E_enc_size;
+        [ rewrite <- e1 in Enc_byte1 | rewrite <- e2 in Enc_byte1 |  rewrite <- e3 in Enc_byte1 | rewrite <- e4 in Enc_byte1 ];
+        subst;
+        unfold codepoint_range_to_codepoint, bind in Parse_lesser; simpl in Parse_lesser.
+      * inversion Parse_lesser. subst. clear Parse_lesser.
+        rewrite <- many_aux_saturation_aux with (n:= (S (Datatypes.length (Byte.of_bits (b1, (b2, (b3, (b4, (b5, (b6, (b7, false))))))) :: rest1)))) in IH_bytes; [ | apply parse_codepoint_strong_progress | simpl; lia |  simpl; lia ].
+        fold (many parse_codepoint rest1) in IH_bytes. fold (utf8_decode rest1) in IH_bytes.
+        destruct (utf8_decode rest1) as [[val rest2] | err] eqn:U_rest1; [| discriminate IH_bytes ].
+        inversion IH_bytes; apply IHbytes in U_rest1; subst. unfold utf8_encode, map. fold (map utf8_encode_codepoint). unfold concat. fold (concat (map utf8_encode_codepoint val)).
+        unfold utf8_encode_codepoint, b4_zero; reflexivity. simpl in enough_fuel. lia.
+      * destruct (parse_continuation bytes_rest1) as [[[[[[[b6 b5] b4] b3] b2] b1] bytes_rest2] | err] eqn: Parse_bytes_rest1; [ | discriminate Parse_lesser].
+        no_overlong_encoding Parse_lesser; inversion Parse_lesser; subst; clear Parse_lesser;
+        apply parse_continuation_strong_progress in Parse_bytes_rest1 as bytes_rest1_len;
+        rewrite <- many_aux_saturation_aux with (n:= S (S (Datatypes.length bytes_rest1))) in IH_bytes; try apply parse_codepoint_strong_progress; try (simpl; lia);
+        fold (many parse_codepoint rest1) in IH_bytes; fold (utf8_decode rest1) in IH_bytes;
+        destruct (utf8_decode rest1) as [[val rest2] | err] eqn:U_rest1; try discriminate IH_bytes;
+        inversion IH_bytes; apply IHbytes in U_rest1; subst; unfold utf8_encode, map; fold (map utf8_encode_codepoint); unfold concat; fold (concat (map utf8_encode_codepoint val));
+        unfold utf8_encode_codepoint, b4_zero; fold utf8_encode_codepoint;
+          destruct_parse_continuation; simpl in Parse_bytes_rest1; inversion Parse_bytes_rest1; subst;
+          try reflexivity; simpl in enough_fuel; lia. 
+      * destruct (parse_continuation bytes_rest1) as [[[[[[[b12 b11] b10] b9] b8] b7] bytes_rest2] | err] eqn: Parse_bytes_rest1; [ | discriminate Parse_lesser].
+        destruct (parse_continuation bytes_rest2) as [[[[[[[b6 b5] b4] b3] b2] b1] bytes_rest3] | err] eqn: Parse_bytes_rest2; [ | discriminate Parse_lesser].
+        no_overlong_encoding Parse_lesser; inversion Parse_lesser; subst; clear Parse_lesser;
+          apply parse_continuation_strong_progress in Parse_bytes_rest1 as bytes_rest1_len;
+          apply parse_continuation_strong_progress in Parse_bytes_rest2 as bytes_rest2_len;
+          rewrite <- many_aux_saturation_aux with (n:= S (S (Datatypes.length bytes_rest1))) in IH_bytes; try apply parse_codepoint_strong_progress; try (simpl; lia);
+          fold (many parse_codepoint rest1) in IH_bytes; fold (utf8_decode rest1) in IH_bytes; 
+          destruct (utf8_decode rest1) as [[val rest2] | err] eqn:U_rest1; try discriminate IH_bytes;
+          inversion IH_bytes; apply IHbytes in U_rest1; subst; unfold utf8_encode, map; fold (map utf8_encode_codepoint); unfold concat; fold (concat (map utf8_encode_codepoint val)); repeat destruct_parse_continuation;
+          unfold utf8_encode_codepoint, b4_zero; fold utf8_encode_codepoint; inversion Parse_bytes_rest2; inversion Parse_bytes_rest1; subst; try reflexivity; simpl in enough_fuel; lia.
+        * destruct (parse_continuation bytes_rest1) as [[[[[[[b18 b17] b16] b15] b14] b13] bytes_rest2] | err] eqn: Parse_bytes_rest1; [ | discriminate Parse_lesser].
+          destruct (parse_continuation bytes_rest2) as [[[[[[[b12 b11] b10] b9] b8] b7] bytes_rest3] | err] eqn: Parse_bytes_rest2; [ | discriminate Parse_lesser].
+          destruct (parse_continuation bytes_rest3) as [[[[[[[b6 b5] b4] b3] b2] b1] bytes_rest4] | err] eqn: Parse_bytes_rest3; [ | discriminate Parse_lesser].
+          apply parse_continuation_strong_progress in Parse_bytes_rest1 as bytes_rest1_len;
+            apply parse_continuation_strong_progress in Parse_bytes_rest2 as bytes_rest2_len;
+            apply parse_continuation_strong_progress in Parse_bytes_rest3 as bytes_rest3_len;
+          rewrite <- many_aux_saturation_aux with (n:= S (S (Datatypes.length bytes_rest1))) in IH_bytes;
+            [ | apply parse_codepoint_strong_progress | | ];
+            try (no_overlong_encoding Parse_lesser; inversion Parse_lesser; simpl; simpl in enough_fuel; subst; lia).
+          fold (many parse_codepoint rest1) in IH_bytes; fold (utf8_decode rest1) in IH_bytes.
+          destruct (utf8_decode rest1) as [[val2 rest2] | err] eqn:U_rest1; try discriminate IH_bytes.
+          repeat destruct_parse_continuation. inversion Parse_bytes_rest1; inversion Parse_bytes_rest2; inversion Parse_bytes_rest3; subst.
+          inversion IH_bytes; apply IHbytes in U_rest1;
+            no_overlong_encoding Parse_lesser; inversion Parse_lesser; subst; clear Parse_lesser; subst;
+            try (simpl in *; lia);
+            unfold utf8_encode, map; fold (map utf8_encode_codepoint); unfold concat; fold (concat (map utf8_encode_codepoint val2)); try reflexivity.
+Defined.
+
 Theorem decode_encode_correct: forall (unicode: unicode_str) (bytes rest: list Byte.byte),
     (utf8_decode bytes = Ok (unicode, rest)) ->
     bytes = List.app (utf8_encode unicode) rest.
 Proof.
-  Admitted.
-  
-  (* intros unicode bytes. *)
-  (* destruct encoding_size_correct as [enc_one [enc_two [enc_three enc_four]]]. *)
-  (* generalize dependent unicode. *)
-  (* induction bytes as [ | byte1 bytes_rest]; intros. *)
-  (* - inversion H. reflexivity. *)
-  (* - unfold utf8_decode, many in H. *)
-  (*   unfold many_aux in H. fold (@many_aux codepoint) in H. unfold bind in H. *)
-  (*   destruct (parse_codepoint (byte1 :: bytes_rest)) as [[val rest'] | err] eqn:ParseByte1; *)
-  (*     [ | inversion H; subst; unfold utf8_encode; reflexivity ]. *)
-    
-  (*   rewrite <- many_aux_saturation_aux with (n:= (Datatypes.length (byte1 :: bytes_rest))) in H. *)
-  (*   2: { apply parse_codepoint_strong_progress. } *)
-  (*   fold (@many codepoint Byte.byte unicode_error parse_codepoint rest') in H. fold (utf8_decode rest') in H. *)
-  (*   destruct (utf8_decode rest') as [[u r] | err]; try discriminate H. inversion H. subst. clear H. *)
-  (*   unfold parse_codepoint, parse_header in ParseByte1. *)
-  (*   destruct (encoding_size_from_header byte1) as [ enc_size | ] eqn:E_enc_size_byte1. *)
-  (*   + unfold bind in ParseByte1. destruct enc_size eqn:E_enc_size. *)
-  (*     * simpl in ParseByte1. *)
-  (*       destruct b as [[[[[[b1 b2] b3] b4] b5] b6] b7]. inversion ParseByte1. *)
-  (*       erewrite <- enc_one in E_enc_size_byte1. *)
-  (*       unfold utf8_encode. *)
-        
-  (* intros unicode. *)
-  (* induction unicode; intros. *)
-  (* - unfold utf8_decode in H. simpl. *)
-  (*   generalize dependent rest. *)
-  (*   induction bytes; intros; unfold many in H; simpl in H. *)
-  (*   + inversion H. reflexivity. *)
-  (*   + destruct (parse_codepoint (a::bytes)) as [[val1 rest1] | err1]; try discriminate H. *)
-  (*     destruct (parse_codepoint rest1) as [[val2 rest2] | err2]; try discriminate H. *)
-  (*     destruct (many_aux parse_codepoint (Datatypes.length bytes) rest2) as [[val3 rest3] | err3]; discriminate H. *)
-  (*     inversion H. reflexivity. *)
-  (* - unfold utf8_decode in H. *)
-    
-      
-    
-   
-
-  
+  intros.
+  apply decode_encode_correct_strong with (bytes:= bytes). lia. apply H.
+Defined.
